Playing some more.

cptd-ssr/cpdt-chapter8.v
@@ -3,22 +3,14 @@ Set Implicit Arguments.
 Unset Strict Implicit.
 Unset Printing Implicit Defensive.
 
-Inductive type : Set := Nat | Bool | Prod of type & type. 
+Inductive type := Nat | Bool | Prod of type & type. 
 
-(*
-Inductive exp : type -> Set :=
-| NConst : nat -> exp Nat
-| Plus : exp Nat -> exp Nat -> exp Nat
-| Eq : exp Nat -> exp Nat -> exp Bool
-
-| BConst : bool -> exp Bool
-| And : exp Bool -> exp Bool -> exp Bool
-| If : forall t, exp Bool -> exp t -> exp t -> exp t
-
-| Pair : forall t1 t2, exp t1 -> exp t2 -> exp (Prod t1 t2)
-| Fst : forall t1 t2, exp (Prod t1 t2) -> exp t1
-| Snd : forall t1 t2, exp (Prod t1 t2) -> exp t2.
-*)
+Fixpoint typeDenote t :=
+  match t with
+    Nat => nat
+  | Bool => bool
+  | Prod t1 t2 => prod (typeDenote t1) (typeDenote t2)
+  end.
 
 Inductive exp t := 
   NConst' of Nat = t & nat
@@ -38,8 +30,8 @@ Notation BConst := (BConst' (erefl _)).
 Notation And := (And' (erefl _)).
 Notation Pair := (Pair' (erefl _)).
 
-(* a better induction principle, to gather the like constructors *)
-(* and remove unnecessary type equations *)
+(* a better induction principle; gathers the like constructors *)
+(* and removes unnecessary type equations *)
 
 Lemma exp_ind' (P : forall t : type, exp t -> Prop) : 
         [/\ forall n, P Nat (NConst n) &
@@ -62,42 +54,48 @@ Lemma eqc T t (r : t = t) (e : T t) : cast r e = e.
 Proof. by move: r; apply: Streicher_K. Qed.
 
 (*
-(* re-introducing casts *)
-Lemma recast T t t' (P : forall t, t' = t -> T t) (r : t' = t) : 
-        P t r = cast r (P t' (erefl _)).
-Proof. by move: (r); rewrite -r; apply: Streicher_K. Qed.
+(* One can recover the behavior of the family as follows *)
 
-(* better case analysis over exp t that *)
-(* doesn't go down to primed constructors *)
-(* this is a boring boilerplate, which is in Coq done by tactics *)
-(* but let's not use tactics here *)
-
-Inductive exp_spec t : exp t -> Type := 
-| nconst_exp n : Nat = t -> forall pf, exp_spec (cast pf (NConst n)) 
-| plus_exp e1 e2 : Nat = t -> forall pf, exp_spec (cast pf (Plus e1 e2))
-| eq_exp e1 e2 : Bool = t -> forall pf, exp_spec (cast pf (Eq e1 e2))
-| bconst_exp b : Bool = t -> forall pf, exp_spec (cast pf (BConst b))
-| and_exp e1 e2 : Bool = t -> forall pf, exp_spec (cast pf (And e1 e2))
-| if_exp b (e1 e2 : exp t) : exp_spec (If b e1 e2)
+Inductive exp_spec : forall t', exp t' -> Type := 
+  nconst_exp n : exp_spec (NConst n)
+| plus_exp e1 e2 : exp_spec (Plus e1 e2)
+| eq_exp e1 e2 : exp_spec (Eq e1 e2)
+| bconst_exp b : exp_spec (BConst b)
+| and_exp e1 e2 : exp_spec (And e1 e2)
+| if_exp t b (e1 e2 : exp t) : exp_spec (If b e1 e2)
 | pair_exp t1 t2 (e1 : exp t1) (e2 : exp t2) : 
-    Prod t1 t2 = t -> forall pf, exp_spec (cast pf (Pair e1 e2))
-| fst_exp t2 (e : exp (Prod t t2)) : exp_spec (Fst e)
-| snd_exp t1 (e : exp (Prod t1 t)) : exp_spec (Snd e).
+    exp_spec (Pair e1 e2)
+| fst_exp t t2 (e : exp (Prod t t2)) : exp_spec (Fst e)
+| snd_exp t t1 (e : exp (Prod t1 t)) : exp_spec (Snd e).
 
 Lemma expP t (e : exp t) : exp_spec e.
-Proof. case: e=>*. rewrite 1?(recast (fun t => _)); constructor. Qed.
+Proof. by case: e=>*; try subst t; constructor. Qed.
 
-(* test goal *)
-Lemma xx n (x : exp Nat) : x = NConst n.
-Proof. case/expP: x=>//. Abort.
+(*
+Given t : type, x : exp t, casing over (expP x) will rewrite
+occurences of x in the goal by NConst n, Plus e1 e2, etc, and the
+occurences of t by Nat, Nat, Bool, etc, as it corresponds.
+
+Very often this results in ill-typed goals, so one needs to use
+occurence selectors and patterns to prevent some occurence from being
+changed.
 *)
 
-Fixpoint typeDenote (t : type) : Set :=
-  match t with
-    Nat => nat
-  | Bool => bool
-  | Prod t1 t2 => prod (typeDenote t1) (typeDenote t2)
-  end.
+(* test goals *)
+Lemma xx1 n (x : exp Nat) : x = NConst n.
+Proof. 
+case: {-1}Nat x / (expP x) (erefl _). 
+(* the above works, because we protected the first occurence of pattern Nat
+(which is what t is in this case, from being changed. But all the other occurences
+are changed. Notice also that we had to first abstract erefl, as the first
+occurence of Nat is precisely in the type of the erefl *)
+Abort.
+
+Lemma xx2 t (x : exp t) : t = Nat /\ x = x.
+Proof. 
+case: {-1}t x / (expP x).
+Abort.
+*)
 
 Fixpoint expDenote t (e : exp t) : typeDenote t :=
   match e with
@@ -112,42 +110,39 @@ Fixpoint expDenote t (e : exp t) : typeDenote t :=
   | Snd _ e' => snd (expDenote e')
   end.
 
-Lemma fst_out t1 t2 s1 s2 : Prod t1 t2 = Prod s1 s2 -> t1 = s1.
-Proof. by case. Defined.
-
-Lemma snd_out t1 t2 s1 s2 : Prod t1 t2 = Prod s1 s2 -> t2 = s2.
+Lemma pair_out t1 t2 s1 s2 : Prod t1 t2 = Prod s1 s2 -> t1 = s1 /\ t2 = s2.
 Proof. by case. Qed.
 
 Fixpoint cfold t (e : exp t) : exp t :=
   match e with
     NConst' r n => NConst' r n
   | Plus' r e1 e2 => 
-      let: (e1', e2') := (cfold e1, cfold e2) in
-      if (e1', e2') is (NConst' _ n1, NConst' _ n2) then NConst' r (n1 + n2)
-      else Plus' r e1' e2'
+      let: (f1, f2) := (cfold e1, cfold e2) in
+      if (f1, f2) is (NConst' _ n1, NConst' _ n2) then NConst' r (n1 + n2)
+      else Plus' r f1 f2
   | Eq' r e1 e2 =>
-      let: (e1', e2') := (cfold e1, cfold e2) in
-      if (e1', e2') is (NConst' _ n1, NConst' _ n2) then BConst' r (n1 == n2) 
-      else Eq' r e1' e2' 
+      let: (f1, f2) := (cfold e1, cfold e2) in
+      if (f1, f2) is (NConst' _ n1, NConst' _ n2) then BConst' r (n1 == n2) 
+      else Eq' r f1 f2 
   | BConst' r b => BConst' r b
   | And' r e1 e2 =>
-      let: (e1', e2') := (cfold e1, cfold e2) in
-      if (e1', e2') is (BConst' _ b1, BConst' _ b2) then BConst' r (b1 && b2)
-      else And' r e1' e2' 
+      let: (f1, f2) := (cfold e1, cfold e2) in
+      if (f1, f2) is (BConst' _ b1, BConst' _ b2) then BConst' r (b1 && b2)
+      else And' r f1 f2 
   | If e e1 e2 =>
-      let: e' := cfold e in
-      match e' with
+      let: f := cfold e in
+      match f with
         BConst' _ true => cfold e1
       | BConst' _ false => cfold e2
-      | _ => If e' (cfold e1) (cfold e2)
+      | _ => If f (cfold e1) (cfold e2)
       end
   | Pair' _ _ r e1 e2 => Pair' r (cfold e1) (cfold e2) 
   | Fst _ e =>
-      let: e' := cfold e in
-      if e' is Pair' _ _ r e1 e2 then cast (fst_out r) e1 else Fst e'
+      let: f := cfold e in
+      if f is Pair' _ _ r e1 e2 then cast (proj1 (pair_out r)) e1 else Fst f
   | Snd _ e =>
-      let e' := cfold e in
-      if e' is Pair' _ _ r e1 e2 then cast (snd_out r) e2 else Snd e'
+      let f := cfold e in
+      if f is Pair' _ _ r e1 e2 then cast (proj2 (pair_out r)) e2 else Snd f
   end. 
 
 Lemma cfold_correct t (e : exp t) : expDenote e = expDenote (cfold e).
@@ -159,73 +154,84 @@ elim/exp_ind': e=>//=.
 by split=>??? ->; case: (cfold _)=>//= ?? r; case: r (r)=>->-> *; rewrite !eqc.
 Qed.
 
+(* Implementation using an indexed family *)
 
+Inductive exp2 : type -> Type :=
+  NConst2 of nat : exp2 Nat
+| Plus2 of exp2 Nat & exp2 Nat : exp2 Nat
+| Eq2 of exp2 Nat & exp2 Nat : exp2 Bool
+| BConst2 of bool : exp2 Bool
+| And2 of exp2 Bool & exp2 Bool : exp2 Bool
+| If2 t of exp2 Bool & exp2 t & exp2 t : exp2 t
+| Pair2 t1 t2 of exp2 t1 & exp2 t2 : exp2 (Prod t1 t2)
+| Fst2 t1 t2 of exp2 (Prod t1 t2) : exp2 t1
+| Snd2 t1 t2 of exp2 (Prod t1 t2) : exp2 t2.
 
-
-Definition pairOutType (t : type) := option (if t is Prod t1 t2 then exp t1 * exp t2 else unit).
-
-Definition pairOut t (e : exp t) :=
-  match e in (exp t) return (pairOutType t) with
-    | Pair _ _ e1 e2 => Some (e1, e2)
-    | _ => None
+Fixpoint expDenote2 t (e : exp2 t) : typeDenote t :=
+  match e with
+    NConst2 n => n
+  | Plus2 e1 e2 => expDenote2 e1 + expDenote2 e2
+  | Eq2 e1 e2 => expDenote2 e1 == expDenote2 e2
+  | BConst2 b => b
+  | And2 e1 e2 => expDenote2 e1 && expDenote2 e2
+  | If2 _ e' e1 e2 => if expDenote2 e' then expDenote2 e1 else expDenote2 e2
+  | Pair2 _ _ e1 e2 => (expDenote2 e1, expDenote2 e2)
+  | Fst2 _ _ e' => fst (expDenote2 e')
+  | Snd2 _ _ e' => snd (expDenote2 e')
   end.
 
-Fixpoint cfold t (e : exp t) : exp t :=
+Definition pairOutType t := 
+  option (if t is Prod t1 t2 then exp2 t1 * exp2 t2 else unit).
+
+Definition pair_out2 t (e : exp2 t) :=
+  if e is Pair2 _ _ e1 e2 in exp2 t return pairOutType t 
+  then Some (e1, e2) else None. 
+
+Fixpoint cfold2 t (e : exp2 t) : exp2 t :=
   match e with
-    | NConst n => NConst n
-    | Plus e1 e2 =>
-      let e1' := cfold e1 in
-      let e2' := cfold e2 in
-      match e1', e2' return exp Nat with
-        | NConst n1, NConst n2 => NConst (n1 + n2)
-        | _, _ => Plus e1' e2'
+    NConst2 n => NConst2 n
+  | Plus2 e1 e2 =>
+      let: (f1, f2) := (cfold2 e1, cfold2 e2) in
+      if (f1, f2) is (NConst2 n1, NConst2 n2) then NConst2 (n1 + n2)
+      else Plus2 f1 f2
+  | Eq2 e1 e2 =>
+      let: (f1, f2) := (cfold2 e1, cfold2 e2) in
+      if (f1, f2) is (NConst2 n1, NConst2 n2) then BConst2 (n1 == n2)
+      else Eq2 f1 f2
+  | BConst2 b => BConst2 b
+  | And2 e1 e2 =>
+      let: (f1, f2) := (cfold2 e1, cfold2 e2) in
+      if (f1, f2) is (BConst2 b1, BConst2 b2) then BConst2 (b1 && b2)
+      else And2 f1 f2
+  | If2 _ e e1 e2 =>
+      let: f := cfold2 e in
+      match f with
+        BConst2 true => cfold2 e1
+      | BConst2 false => cfold2 e2
+      | _ => If2 f (cfold2 e1) (cfold2 e2)
       end
-    | Eq e1 e2 =>
-      let e1' := cfold e1 in
-      let e2' := cfold e2 in
-      match e1', e2' return exp Bool with
-        | NConst n1, NConst n2 => BConst (n1 == n2)
-        | _, _ => Eq e1' e2'
-      end
-
-    | BConst b => BConst b
-    | And e1 e2 =>
-      let e1' := cfold e1 in
-      let e2' := cfold e2 in
-      match e1', e2' return exp Bool with
-        | BConst b1, BConst b2 => BConst (b1 && b2)
-        | _, _ => And e1' e2'
-      end
-    | If _ e e1 e2 =>
-      let e' := cfold e in
-      match e' with
-        | BConst true => cfold e1
-        | BConst false => cfold e2
-        | _ => If e' (cfold e1) (cfold e2)
-      end
-
-    | Pair _ _ e1 e2 => Pair (cfold e1) (cfold e2)
-    | Fst _ _ e =>
-      let e' := cfold e in
-      match pairOut e' with
-        | Some p => fst p
-        | None => Fst e'
-      end
-    | Snd _ _ e =>
-      let e' := cfold e in
-      match pairOut e' with
-        | Some p => snd p
-        | None => Snd e'
-      end
+  | Pair2 _ _ e1 e2 => Pair2 (cfold2 e1) (cfold2 e2)
+  | Fst2 _ _ e =>
+      let: f := cfold2 e in
+      if pair_out2 f is Some p then fst p else Fst2 f
+  | Snd2 t1 t2 e1 =>
+      let: f := cfold2 e1 in
+      if pair_out2 f is Some p then snd p else Snd2 f
 end.
 
-Theorem cfold_correct t (e : exp t): expDenote e = expDenote (cfold e).
+Lemma cfold_correct2 t (e : exp2 t) : expDenote2 e = expDenote2 (cfold2 e).
 Proof.
-elim:e=>//. move=>e1 H1 e2 H2.
-- rewrite [cfold _]/=.
-  case: e1.
-
-- simpl. case: e1.
-
-
-move: (@expDenote Nat e1) (@expDenote Nat e2) H1 H2.
+elim: e=>//. 
+- move=>/= e1 -> e2 ->. 
+Set Printing All.
+(* in this goal, it's really impossible to count the occurences *)
+(* moreover, the casing will change Nat to other types, but I have *)
+(* addition in the goal, which will thus always be ill-typed after casing *)
+(* it's not clear that that can even be protected by an occurence selection *)
+(* hence, i don't think the right first move here is to case *)
+(* rather, one has to obtain some type equations first, maybe by *)
+(* inversion, or some other tactic *)
+(* in principle, this whole approach looks completely wrongheaded *)
+try case: {-3}Nat / (cfold2 e1).
+Unset Printing All.
+Abort.
